decomposing call_end and call_e

Hoare/PathInvariant.thy
@@ -148,7 +148,7 @@ using ncall_stack_length call_ncall
 
 (* because the pushed element didn't change, current must have the
    invariant, and we can use the mono push rule *)
-lemma call_invariant :
+lemma call_mono_invariant :
   "call (map snd lst) \<Longrightarrow>
    monoI iv (hd lst) \<Longrightarrow>
    pathR (mono_rules iv) lst \<Longrightarrow>
@@ -189,6 +189,272 @@ defer
 apply (simp add: take_map)
 apply (auto simp add:pathR_take)
   by (metis One_nat_def Suc_1 Suc_diff_Suc Suc_lessD diff_Suc_less hd_take last_take)
+
+lemma call_first_prev :
+"call_end lst (last lst) \<Longrightarrow>
+ last (take (length lst - Suc 0) lst) = lst!0"
+  by (smt Nitpick.size_list_simp(2) One_nat_def Suc_diff_Suc call_end_def diff_Suc_Suc diff_less first_one_smaller_prev last_take length_tl less_numeral_extra(2) zero_less_Suc)
+
+lemma decompose_call_end :
+  "call_end lst (last lst) \<Longrightarrow>
+   x \<in> set (indexSplit (findIndices (take (length lst-1) lst) (lst!0))
+             (take (length lst-1) lst)) \<Longrightarrow>
+   call_end x (lst!0) \<or> const_seq x (lst!0)"
+using correct_pieces [of "take (length lst-1) lst" x]
+apply simp
+apply (subgoal_tac "inc_decL (take (length lst - 1) lst)")
+defer
+apply (simp add:pathR_take call_end_def inc_decL_def)
+apply simp
+apply (subgoal_tac "lst \<noteq> [] \<and> 1 < length lst")
+defer
+apply (simp add:call_end_def)
+  using less_nat_zero_code apply auto[1]
+apply clarsimp
+apply (subgoal_tac "hd (take (length lst - Suc 0) lst) = lst!0")
+defer
+  apply (simp add: hd_conv_nth)
+apply simp
+apply (subgoal_tac "last (take (length lst - Suc 0) lst) = lst!0")
+defer
+using call_first_prev apply fastforce
+apply (simp add:split_def)
+  by (metis One_nat_def call_end_def first_smaller1 first_smaller_before)
+
+lemma decompose_call_end_index :
+  "call_end lst (last lst) \<Longrightarrow>
+   \<exists>ilst. (\<forall>x \<in> set (indexSplit ilst (take (length lst-1) lst)).
+   call_end x (lst!0) \<or> const_seq x (lst!0))"
+apply (rule exI[where x =
+   "findIndices (take (length lst-1) lst) (lst!0)"])
+using decompose_call_end apply fastforce
+done
+
+lemma call_e_end :
+"call_e lst (last lst) \<Longrightarrow>
+ call_end (map length lst) (last (map length lst))"
+  using call_end1 call_end_last by fastforce
+
+lemma call_e_pathR:
+"call_e lst (last lst) \<Longrightarrow> pathR push_pop lst"
+by (simp add:call_e_def push_popL_def)
+
+(*
+lemma call_end_inside_big_idx :
+"call_end lst (last lst) \<Longrightarrow>
+ j < length lst - 1 \<Longrightarrow>
+ lst ! 0 \<le> lst ! j"
+*)
+
+lemma call_end_inside_big :
+"call_end lst (last lst) \<Longrightarrow>
+ x \<in> set (take (length lst - 1) lst) \<Longrightarrow>
+ lst ! 0 \<le> x"
+using first_smaller1 [of "lst" "length lst - 1"]
+using first_smaller_before [of "length lst -1" "lst" x]
+by (auto simp add:call_end_def sucR_def)
+
+lemma call_e_inside_big_idx :
+"call_e lst (last lst) \<Longrightarrow>
+ j < length lst - 1 \<Longrightarrow>
+ takeLast (length (lst!0)) (lst!j) = lst ! 0"
+using stack_unchanged [of "take (Suc j) lst"
+   "length (lst!0)"]
+apply simp
+apply (cases "push_popL (take (Suc j) lst)")
+defer
+apply (simp add:call_e_def push_popL_def pathR_take)
+apply (cases "take (Suc j) lst = []")
+apply (simp add:clip_def call_e_def)
+
+apply (simp add:last_take hd_take)
+apply (subgoal_tac "\<forall>sti\<in>set (take (Suc j)lst).
+        length (lst ! 0) \<le> length sti")
+apply auto
+  apply (simp add: hd_conv_nth)
+
+subgoal for sti
+using call_end_inside_big [of "map length lst" "length sti"]
+apply (simp add:call_e_end)
+apply (cases "length sti
+     \<in> set (take (length (map length lst) - 1) (map length lst))")
+apply auto
+  apply (simp add: clip_def drop_map take_map)
+  by (meson Suc_leI image_eqI set_take_subset_set_take subset_code(1))
+done
+
+lemma call_e_inside_big :
+ "call_e lst (last lst) \<Longrightarrow>
+  a \<in> set (take (length lst - 1) lst) \<Longrightarrow>
+  takeLast (length (lst ! 0)) a = lst ! 0"
+using ex_idx [of a "take (length lst - 1) lst"]
+by (auto simp add: call_e_inside_big_idx)
+
+(* decompose call_e into smaller pieces ... should follow from
+   above similarly to call decomposition *)
+lemma decompose_call_e_index :
+  "call_e lst (last lst) \<Longrightarrow>
+   \<exists>ilst. (\<forall>x \<in> set (indexSplit ilst (take (length lst-1) lst)).
+   call_e x (lst!0) \<or> const_seq x (lst!0))"
+using decompose_call_end_index [of "map length lst"]
+      call_e_end [of lst]
+apply auto
+subgoal for ilst
+apply (rule exI[where x=ilst])
+apply clarsimp
+(* because internally the stack is high,
+   it should not change *)
+apply (case_tac "const_seq (map length x) (map length lst ! 0) \<or>
+    call_end (map length x) (map length lst ! 0)")
+defer
+subgoal for x
+using index_split_map [of x ilst "take (length lst - 1) lst" length]
+apply (simp add:take_map drop_map)
+apply force
+done
+subgoal for x
+using pathR_split [of "push_pop"
+   "take (length lst - 1) lst" x ilst]
+  pathR_take [of "push_pop" lst "length lst-1"]
+  call_e_pathR [of lst]
+apply simp
+
+apply auto
+subgoal (* constant *)
+using const_seq_convert [of x "map length lst ! 0"]
+apply (auto simp add:push_popL_def)
+apply (cases x)
+using const_seq_empty apply force
+subgoal for xa a list
+apply (simp add:map_nth)
+using const_seq_eq [of a list xa]
+apply simp
+apply (subgoal_tac "a \<in> set (take (length lst - 1) lst)")
+defer
+using in_index_split apply fastforce
+apply (subgoal_tac "lst ! 0 = a")
+apply auto
+
+using call_e_inside_big [of lst a]
+  by (metis One_nat_def PathRel.take_all const_seq_eq length_greater_0_conv length_pos_if_in_set nth_map take_eq_Nil)
+done
+apply (rule call_end2)
+  apply (clarsimp simp add: call_e_def)
+  apply (metis Suc_lessD nth_map)
+
+  using push_popL_def apply blast
+using call_end_last [of "map length x" "length (lst ! 0)"]
+using call_e_inside_big [of lst "last x"]
+apply simp
+apply (subgoal_tac "map length lst ! 0 = length (lst!0)")
+defer
+apply (simp add:call_e_def)
+  using Suc_lessD nth_map apply blast
+apply simp
+apply (subgoal_tac "last x \<in> set (take (length lst - 1) lst)")
+defer
+apply (rule in_index_split [of x ilst "take (length lst-1) lst"
+  "last x"])
+apply auto
+apply (simp add:call_end_def)
+  apply (metis One_nat_def Suc_lessD diff_Suc_less gr_implies_not_zero in_set_conv_nth last_conv_nth length_0_conv)
+apply (subgoal_tac "length (last x) = length (lst!0)")
+  apply (metis PathRel.take_all)
+apply (simp add:call_end_def)
+  by (metis Suc_lessD last_map length_greater_0_conv)
+done done
+
+lemma decompose_call_e :
+  "call_e lst (last lst) \<Longrightarrow>
+  ilst = findIndices
+             (take (length lst - Suc 0)
+               (map length lst))
+             (map length lst ! 0) \<Longrightarrow>
+   x \<in> set (indexSplit ilst (take (length lst-1) lst)) \<Longrightarrow>
+   call_e x (lst!0) \<or> const_seq x (lst!0)"
+using decompose_call_end [of "map length lst" "map length x"]
+      call_e_end [of lst]
+apply auto
+apply (case_tac "const_seq (map length x) (map length lst ! 0) \<or>
+    call_end (map length x) (map length lst ! 0)")
+defer
+using index_split_map [of x ilst "take (length lst - 1) lst" length]
+apply (simp add:take_map drop_map)
+using pathR_split [of "push_pop"
+   "take (length lst - 1) lst" x ilst]
+  pathR_take [of "push_pop" lst "length lst-1"]
+  call_e_pathR [of lst]
+apply simp
+
+apply auto
+subgoal (* constant *)
+using const_seq_convert [of x "map length lst ! 0"]
+apply (auto simp add:push_popL_def)
+apply (cases x)
+using const_seq_empty apply force
+subgoal for xa a list
+apply (simp add:map_nth)
+using const_seq_eq [of a list xa]
+apply simp
+apply (subgoal_tac "a \<in> set (take (length lst - 1) lst)")
+defer
+using in_index_split apply fastforce
+apply (subgoal_tac "lst ! 0 = a")
+apply auto
+
+using call_e_inside_big [of lst a]
+  by (metis One_nat_def PathRel.take_all const_seq_eq length_greater_0_conv length_pos_if_in_set nth_map take_eq_Nil)
+done
+apply (rule call_end2)
+  apply (clarsimp simp add: call_e_def)
+  apply (metis Suc_lessD nth_map)
+
+  using push_popL_def apply blast
+using call_end_last [of "map length x" "length (lst ! 0)"]
+using call_e_inside_big [of lst "last x"]
+apply simp
+apply (subgoal_tac "map length lst ! 0 = length (lst!0)")
+defer
+apply (simp add:call_e_def)
+  using Suc_lessD nth_map apply blast
+apply simp
+apply (subgoal_tac "last x \<in> set (take (length lst - 1) lst)")
+defer
+apply (rule in_index_split [of x ilst "take (length lst-1) lst"
+  "last x"])
+apply auto
+apply (simp add:call_end_def)
+  apply (metis One_nat_def Suc_lessD diff_Suc_less gr_implies_not_zero in_set_conv_nth last_conv_nth length_0_conv)
+apply (subgoal_tac "length (last x) = length (lst!0)")
+  apply (metis PathRel.take_all)
+apply (simp add:call_end_def)
+by (metis Suc_lessD last_map length_greater_0_conv)
+
+
+definition call_inv :: "('a * 'a list \<Rightarrow> bool) \<Rightarrow> ('a * 'a list) list \<Rightarrow> bool" where
+"call_inv iv l =
+   (call_e (map snd l) (snd (last l)) \<longrightarrow> iv (hd l) \<longrightarrow> iv (last l))"
+
+definition stay_rel :: "('a * 'a list \<Rightarrow> bool) \<Rightarrow> ('a * 'a list) rel" where
+"stay_rel iv = {(a,b) | a b. length (snd a) = length (snd b) \<and> (iv a \<longrightarrow> iv b) }
+             \<union> {(a,b) | a b. length (snd a) \<noteq> length (snd b)}"
+
+definition psublists :: "'a list \<Rightarrow> 'a list set" where
+"psublists lst = {take l (drop i lst) | l i. l < length lst}"
+
+definition callout_rel :: "('a * 'a list \<Rightarrow> bool) \<Rightarrow> nat \<Rightarrow> ('a * 'a list) rel" where
+"callout_rel iv level =
+    {(a,b) | a b. length (snd a) = level \<and> length (snd b) = level + 1 \<and> (iv a \<longrightarrow> iv b) }
+  \<union> {(a,b) | a b. length (snd a) \<noteq> level \<or> length (snd b) \<noteq> level + 1}"
+
+lemma call_invariant :
+  "\<forall>l \<in> psublists lst. call_inv iv l \<Longrightarrow> 
+   pathR (stay_rel iv) lst \<Longrightarrow>
+   (* exit must be good *)
+   (iv (lst!(length lst-2)) \<Longrightarrow> iv (last lst)) \<Longrightarrow>
+   (* call outs should be good *)
+   pathR (callout_rel iv (length (snd (hd lst)))) lst \<Longrightarrow>
+   call_inv iv lst"
 
 
 end
